Prove induction principle for term_traverse
Cant use equations because of bug with monadic binders
Change definition to include equality proof for induction
Prove rewrite and irrelevance lemma for term_traverse
Prove rewrite and induction lemmas for tm_traverse

src/core/TermTraverse.v
@@ -1,6 +1,8 @@
 Require Import Monads TermDefs TermFuncs TermTraverseAux.
 Import MonadNotations.
 Local Open Scope errst_scope.
+Require Import FunctionalExtensionality.
+
 
 (*A traversal function*)
 
@@ -22,6 +24,8 @@ Section Traverse.
 Variable (St: Type). (*The type of state*)
 Variable (R: Type). (*Return type*)
 
+(*NOTE: removing term from these cases, then dont have to carry around.
+  Can carry around type if we want or else calculate for app case*)
 
 Notation T := (errState (CoqBigInt.t * St) R).
 
@@ -45,91 +49,366 @@ Variable (not_case: forall (tm: term_c) (t: term_c) (r: R), T).
 Variable (true_case: term_c ->T).
 Variable (false_case : term_c ->T).
 
-(*This is annoying for sure*)
-
-
 (*We can't use Equations because it doesn't support mutual well-founded
   definitions. So we will use Xavier trick again*)
-
-
-Fixpoint term_traverse (tm1: term_c) (ACC: Acc lt (term_size tm1)) : T :=
+Definition termp := 0.
+Definition term_size_eq' t := eq_sym (term_size_eq t).
+(*For induction, it is useful to generalize proof. This is annoying; we need it in every case although
+  it is always the same proof*)
+Fixpoint term_traverse (tm1: term_c) (ACC: Acc lt (term_size tm1))
+  (Heq: term_node_size (t_node_of tm1) = term_size tm1) : T :=
   match (t_node_of tm1) as t1 return term_node_size t1 = term_size tm1 -> _ with
   | Tconst c => fun _ => const_case tm1 c
   | Tvar x => fun _ => var_case tm1 x
   | Tif t1 t2 t3 => fun Hsz =>
-    v1 <- term_traverse t1 (Acc_inv ACC (tif_size1 Hsz)) ;;
-    v2 <- term_traverse t2 (Acc_inv ACC (tif_size2 Hsz)) ;;
-    v3 <- term_traverse t3 (Acc_inv ACC (tif_size3 Hsz)) ;;
+    v1 <- term_traverse t1 (Acc_inv ACC (tif_size1 Hsz)) (term_size_eq' t1) ;;
+    v2 <- term_traverse t2 (Acc_inv ACC (tif_size2 Hsz)) (term_size_eq' t2) ;;
+    v3 <- term_traverse t3 (Acc_inv ACC (tif_size3 Hsz)) (term_size_eq' t3) ;;
     if_case tm1 t1 t2 t3 v1 v2 v3
   | Tlet t1 b => fun Hsz =>
-    v1 <- term_traverse t1 (Acc_inv ACC (tlet_size1 Hsz)) ;;
+    v1 <- term_traverse t1 (Acc_inv ACC (tlet_size1 Hsz)) (term_size_eq' t1) ;;
     (*Need dependent types here to have enough information for the proof*)
     errst_bind_dep (errst_tup1 (errst_lift1 (t_open_bound b)))
       (fun y s Heq => 
-        v2 <- (term_traverse (snd y) (Acc_inv ACC (tlet_size2 Hsz Heq))) ;;
+        v2 <- (term_traverse (snd y) (Acc_inv ACC (tlet_size2 Hsz Heq)) (term_size_eq' (snd y))) ;;
         let_case tm1 t1 v1 (fst y) (snd y) v2)
   | Tapp l ts => fun Hsz =>
     (*Need dependent map for termination proof*)
     recs <- errst_list (@dep_map _ _ (fun t => term_size t < term_size tm1) 
       (fun t1 (Ht1: term_size t1 < term_size tm1) => 
-        term_traverse t1 (Acc_inv ACC Ht1)) ts (tapp_size Hsz)) ;;
+        term_traverse t1 (Acc_inv ACC Ht1) (term_size_eq' t1)) ts (tapp_size Hsz)) ;;
     (app_case tm1 l ts recs)
   (*Case is the trickiest: we need both a dependent map and a dependent bind*)
   | Tcase t1 tbs => fun Hsz =>
-    r1 <- term_traverse t1 (Acc_inv ACC (tmatch_size1 Hsz)) ;;
+    r1 <- term_traverse t1 (Acc_inv ACC (tmatch_size1 Hsz)) (term_size_eq' t1) ;;
     tbs2 <- errst_list (@dep_map _ _ (fun x => term_size (snd x) < term_size tm1)
       (*Idea: For each element in list, use dependent bind and recursively traverse*)
       (fun b (Hx: term_size (snd b) < term_size tm1) =>
         errst_bind_dep (errst_tup1 (errst_lift1 (t_open_branch b)))
           (fun y s Heq =>
-            t2 <- term_traverse (snd y) (Acc_inv ACC (tmatch_size2 Hx Heq)) ;;
+            t2 <- term_traverse (snd y) (Acc_inv ACC (tmatch_size2 Hx Heq)) (term_size_eq' (snd y)) ;;
             errst_ret (y, t2))
         ) tbs (tmatch_size3 Hsz)) ;;
     match_case tm1 t1 r1 tbs2
   | Teps b => fun Hsz =>
     errst_bind_dep (errst_tup1 (errst_lift1 (t_open_bound b)))
       (fun y s Heq => 
-        v <- (term_traverse (snd y) (Acc_inv ACC (teps_size Hsz Heq))) ;;
+        v <- (term_traverse (snd y) (Acc_inv ACC (teps_size Hsz Heq)) (term_size_eq' (snd y))) ;;
         eps_case tm1 (fst y) (snd y) v)
   (*A slight complication from the triggers - need nested dependent match*)
   | Tquant q tq => fun Hsz =>
     (*NOTE: doing bind ... ret, need for proofs even though superflous*)
     errst_bind_dep (errst_tup1 (errst_lift1 (t_open_quant1 tq)))
       (fun (y : list vsymbol * trigger * term_c) s Heq => 
-        v <- (term_traverse (snd y) (Acc_inv ACC (tquant_size1 Hsz Heq))) ;;
+        v <- (term_traverse (snd y) (Acc_inv ACC (tquant_size1 Hsz Heq)) (term_size_eq' (snd y))) ;;
         let vs := fst (fst y) in
         let tr := snd (fst y) in
         let t := snd y in
         (*Then traverse over triggers*)
         v2 <- errst_list (dep_map (fun l1 (Hl1: Forall (fun x => term_size x < term_size tm1) l1) =>
           errst_list (dep_map (fun tr1 (Ht1: term_size tr1 < term_size tm1) => 
-            term_traverse tr1 (Acc_inv ACC Ht1))
+            term_traverse tr1 (Acc_inv ACC Ht1) (term_size_eq' tr1))
             l1 Hl1)) tr (tquant_size_tr Hsz Heq)) ;;
         quant_case tm1 q vs tr v2 t v)
   | Tbinop b t1 t2 => fun Hsz =>
-    r1 <- term_traverse t1 (Acc_inv ACC (tbinop_size1 Hsz)) ;;
-    r2 <- term_traverse t2 (Acc_inv ACC (tbinop_size2 Hsz)) ;;
+    r1 <- term_traverse t1 (Acc_inv ACC (tbinop_size1 Hsz)) (term_size_eq' t1) ;;
+    r2 <- term_traverse t2 (Acc_inv ACC (tbinop_size2 Hsz)) (term_size_eq' t2) ;;
     binop_case tm1 b t1 t1 r1 r2
   | Tnot t1 => fun Hsz =>
-    r1 <- term_traverse t1 (Acc_inv ACC (tnot_size1 Hsz)) ;;
+    r1 <- term_traverse t1 (Acc_inv ACC (tnot_size1 Hsz)) (term_size_eq' t1) ;;
+    not_case tm1 t1 r1
+  | Ttrue => fun _ => true_case tm1
+  | Tfalse => fun _ => false_case tm1
+  end Heq.
+
+
+(*unfolding is bad*)
+Lemma term_traverse_rewrite (tm1: term_c) (ACC: Acc lt (term_size tm1)) Heq:
+  term_traverse tm1 ACC Heq =
+  match (t_node_of tm1) as t1 return term_node_size t1 = term_size tm1 -> _ with
+  | Tconst c => fun _ => const_case tm1 c
+  | Tvar x => fun _ => var_case tm1 x
+  | Tif t1 t2 t3 => fun Hsz =>
+    v1 <- term_traverse t1 (Acc_inv ACC (tif_size1 Hsz)) (term_size_eq' t1) ;;
+    v2 <- term_traverse t2 (Acc_inv ACC (tif_size2 Hsz)) (term_size_eq' t2) ;;
+    v3 <- term_traverse t3 (Acc_inv ACC (tif_size3 Hsz)) (term_size_eq' t3) ;;
+    if_case tm1 t1 t2 t3 v1 v2 v3
+  | Tlet t1 b => fun Hsz =>
+    v1 <- term_traverse t1 (Acc_inv ACC (tlet_size1 Hsz)) (term_size_eq' t1) ;;
+    (*Need dependent types here to have enough information for the proof*)
+    errst_bind_dep (errst_tup1 (errst_lift1 (t_open_bound b)))
+      (fun y s Heq => 
+        v2 <- (term_traverse (snd y) (Acc_inv ACC (tlet_size2 Hsz Heq)) (term_size_eq' (snd y))) ;;
+        let_case tm1 t1 v1 (fst y) (snd y) v2)
+  | Tapp l ts => fun Hsz =>
+    (*Need dependent map for termination proof*)
+    recs <- errst_list (@dep_map _ _ (fun t => term_size t < term_size tm1) 
+      (fun t1 (Ht1: term_size t1 < term_size tm1) => 
+        term_traverse t1 (Acc_inv ACC Ht1) (term_size_eq' t1)) ts (tapp_size Hsz)) ;;
+    (app_case tm1 l ts recs)
+  (*Case is the trickiest: we need both a dependent map and a dependent bind*)
+  | Tcase t1 tbs => fun Hsz =>
+    r1 <- term_traverse t1 (Acc_inv ACC (tmatch_size1 Hsz)) (term_size_eq' t1) ;;
+    tbs2 <- errst_list (@dep_map _ _ (fun x => term_size (snd x) < term_size tm1)
+      (*Idea: For each element in list, use dependent bind and recursively traverse*)
+      (fun b (Hx: term_size (snd b) < term_size tm1) =>
+        errst_bind_dep (errst_tup1 (errst_lift1 (t_open_branch b)))
+          (fun y s Heq =>
+            t2 <- term_traverse (snd y) (Acc_inv ACC (tmatch_size2 Hx Heq)) (term_size_eq' (snd y)) ;;
+            errst_ret (y, t2))
+        ) tbs (tmatch_size3 Hsz)) ;;
+    match_case tm1 t1 r1 tbs2
+  | Teps b => fun Hsz =>
+    errst_bind_dep (errst_tup1 (errst_lift1 (t_open_bound b)))
+      (fun y s Heq => 
+        v <- (term_traverse (snd y) (Acc_inv ACC (teps_size Hsz Heq)) (term_size_eq' (snd y))) ;;
+        eps_case tm1 (fst y) (snd y) v)
+  (*A slight complication from the triggers - need nested dependent match*)
+  | Tquant q tq => fun Hsz =>
+    (*NOTE: doing bind ... ret, need for proofs even though superflous*)
+    errst_bind_dep (errst_tup1 (errst_lift1 (t_open_quant1 tq)))
+      (fun (y : list vsymbol * trigger * term_c) s Heq => 
+        v <- (term_traverse (snd y) (Acc_inv ACC (tquant_size1 Hsz Heq)) (term_size_eq' (snd y))) ;;
+        let vs := fst (fst y) in
+        let tr := snd (fst y) in
+        let t := snd y in
+        (*Then traverse over triggers*)
+        v2 <- errst_list (dep_map (fun l1 (Hl1: Forall (fun x => term_size x < term_size tm1) l1) =>
+          errst_list (dep_map (fun tr1 (Ht1: term_size tr1 < term_size tm1) => 
+            term_traverse tr1 (Acc_inv ACC Ht1) (term_size_eq' tr1))
+            l1 Hl1)) tr (tquant_size_tr Hsz Heq)) ;;
+        quant_case tm1 q vs tr v2 t v)
+  | Tbinop b t1 t2 => fun Hsz =>
+    r1 <- term_traverse t1 (Acc_inv ACC (tbinop_size1 Hsz)) (term_size_eq' t1) ;;
+    r2 <- term_traverse t2 (Acc_inv ACC (tbinop_size2 Hsz)) (term_size_eq' t2) ;;
+    binop_case tm1 b t1 t1 r1 r2
+  | Tnot t1 => fun Hsz =>
+    r1 <- term_traverse t1 (Acc_inv ACC (tnot_size1 Hsz)) (term_size_eq' t1) ;;
+    not_case tm1 t1 r1
+  | Ttrue => fun _ => true_case tm1
+  | Tfalse => fun _ => false_case tm1
+  end Heq.
+Proof. destruct tm1. destruct t; destruct ACC;reflexivity.
+Qed.
+
+Definition tm_traverse (tm1: term_c) : T :=
+  term_traverse tm1 (Wf_nat.lt_wf _) (eq_sym (term_size_eq tm1)).
+
+Set Bullet Behavior "Strict Subproofs".
+
+Lemma tm_size_wf: well_founded (fun t1 t2 => term_size t1 < term_size t2).
+Proof.
+  eapply well_founded_lt_compat with (f:=term_size). auto.
+Defined.
+
+Ltac funext := apply functional_extensionality_dep.
+
+Ltac gen_dep_map :=
+  match goal with |- context [dep_map ?f ?l ?H] => generalize dependent H end.
+
+(*We want to prove an unfolding lemma so that we can express [tm_traverse] in terms
+  of itself with no accessibility proofs (like the Equations rewrite principle).
+  To this this, we first need to prove (inductively) that this definition is irrelevant in
+  the accessibility proof. This requires funext*)
+
+(*Don't need to change Heq, get proof irrelevance by UIP_dec*)
+Lemma term_traverse_irrel t Heq ACC1 ACC2:
+  term_traverse t ACC1 Heq = term_traverse t ACC2 Heq.
+Proof.
+  (*need to generalize for induction*)
+  revert ACC1 ACC2 Heq.
+  induction t using (well_founded_induction tm_size_wf). rename H into IH.
+  intros ACC1 ACC2 Heq.
+  rewrite !(term_traverse_rewrite t).
+  destruct t as [n tyo a loc].
+  destruct n; destruct ACC1; destruct ACC2; auto.
+  - (*Tapp*) simpl.
+    f_equal. f_equal. simpl in *. gen_dep_map.
+    simpl. generalize dependent (S (sum (map term_size l0))).
+    induction l0; simpl; auto. intros n IH a1 a2 _ Hall; inversion Hall; subst; f_equal; auto.
+  - (*Tif*) simpl. (*rewrite to avoid needing funext*)
+    rewrite (IH t) with (ACC2:=(a1 (term_size t) (tif_size1 Heq))) by (simpl; lia).
+    rewrite (IH t0) with (ACC2:=(a1 (term_size t0) (tif_size2 Heq))) by (simpl; lia).
+    rewrite (IH t1) with (ACC2:=(a1 (term_size t1) (tif_size3 Heq))) by (simpl; lia).
+    reflexivity.
+  - (*Tlet*) simpl. destruct p as [[v b] t1]. Opaque t_open_bound. simpl.
+    rewrite (IH t) with (ACC2:=(a1 (term_size t) (tlet_size1 Heq))) by (simpl; lia).
+    (*NOTE: need funext here I think*)
+    f_equal. funext. intros x.
+    f_equal. funext. intros tb. funext. intros s. funext. intros Htb.
+    rewrite (IH (snd tb)) with (ACC2:=(a1 (term_size (snd tb)) (tlet_size2 Heq Htb))); auto.
+    simpl. 
+    eapply @tlet_size2 with (tm:=(mk_term_c (Tlet t (v, b, t1)) tyo a loc))(t1:=t) in Htb; simpl in *; lia.
+  - (*Tcase*) Opaque t_open_branch. simpl.
+    rewrite (IH t) with (ACC2:=(a1 (term_size t) (tmatch_size1 Heq))) by (simpl; lia).
+    (*Combo of let and app essentially*)
+    f_equal. funext. intros x. f_equal. f_equal.
+    (*Again, need to generalize sum*)
+    gen_dep_map. simpl in *. generalize dependent (@tmatch_size2 St (mk_term_c (Tcase t l) tyo a loc)).
+    simpl.
+    generalize dependent (S (term_size t + sum (map (fun x0 : pattern_c * bind_info * term_c => term_size (snd x0)) l))).
+    (*Now general enough for induction*)
+    induction l as [| [[p1 b1] t1] ps IHps]; simpl; auto.
+    intros n IHn a1 a2 _ size_bound Hall. inversion Hall; subst; f_equal; auto.
+    (*Now deal with head bound*)
+    clear IHps.
+    f_equal. funext. intros b2. funext. intros s. funext. intros Heq.
+    rewrite (IHn (snd b2)) with (ACC2:=(a2 (term_size (snd b2)) (size_bound s b2 (p1, b1, t1) (Forall_inv Hall) Heq))); auto.
+    apply dep_bnd_size_branch in Heq. simpl in *; lia.
+  - (*Teps*)
+    simpl. destruct p as [[v b] t1]. f_equal. funext. intros tb. funext. intros s. funext. intros Htb.
+    rewrite (IH (snd tb)) with (ACC2:=(a1 (term_size (snd tb)) (teps_size Heq Htb))); auto.
+    simpl. 
+    eapply @teps_size with (tm:=(mk_term_c (Teps (v, b, t1)) tyo a loc)) in Htb; simpl in *; lia.
+  - (*Tquant*) Opaque t_open_quant1. destruct p as [[[vs1 b1] tr1] t1]. simpl.
+    f_equal. funext. intros tq. funext. intros s. funext. intros Heq1.
+    assert (Htq:=Heq1).
+    apply dep_bnd_size_quant in Htq. simpl in Htq. destruct Htq as [Hszt1 Hsztr1].
+    rewrite (IH (snd tq)) with (ACC2:=(a1 (term_size (snd tq)) (tquant_size1 Heq Heq1))) by (simpl; lia).
+    f_equal.  funext. intros x. f_equal. f_equal.
+    (*Now prove trigger maps equiv*)
+    gen_dep_map. simpl in *.
+    generalize dependent (S(term_size t1 + Datatypes.length tr1 +
+      sum (map (fun l : list term_c => sum (map term_size l)) tr1))).
+    clear. induction (snd (fst tq)) as [| l1 tr1 IHtr]; simpl; auto.
+    intros n IHn a1 a2 _ Hall. inversion Hall as [| ? ? IH1 IH2]; subst; f_equal; auto.
+    (*And do single list*)
+    f_equal.
+    gen_dep_map. clear - IHn. induction l1 as [| x1 t1 IH]; simpl; auto. 
+    intros Hall; inversion Hall; subst; f_equal; auto.
+  - (*Tbinop*) simpl. 
+    rewrite (IH t) with (ACC2:=(a1 (term_size t) (tbinop_size1 Heq))) by (simpl; lia).
+    rewrite (IH t0) with (ACC2:=(a1 (term_size t0) (tbinop_size2 Heq))) by (simpl; lia).
+    reflexivity.
+  - (*Tnot*) simpl.
+    rewrite (IH t) with (ACC2:=(a1 (term_size t) (tnot_size1 Heq))) by (simpl; lia).
+    reflexivity.
+Qed.
+
+
+(*Now we prove the rewrite lemma. This does not require induction on the term
+  (though it does need induction for the nested lists) and just applies
+  the previous lemma repeatedly*)
+Lemma tm_traverse_rewrite (tm1: term_c) :
+  tm_traverse tm1 =
+  match (t_node_of tm1) as t1 return term_node_size t1 = term_size tm1 -> _ with
+  | Tconst c => fun _ => const_case tm1 c
+  | Tvar x => fun _ => var_case tm1 x
+  | Tif t1 t2 t3 => fun Hsz =>
+    v1 <- tm_traverse t1 ;;
+    v2 <- tm_traverse t2 ;;
+    v3 <- tm_traverse t3 ;;
+    if_case tm1 t1 t2 t3 v1 v2 v3
+  | Tlet t1 b => fun Hsz =>
+    v1 <- tm_traverse t1 ;;
+    (*Need dependent types here to have enough information for the proof*)
+    errst_bind_dep (errst_tup1 (errst_lift1 (t_open_bound b)))
+      (fun y s Heq => 
+        v2 <- (tm_traverse (snd y)) ;;
+        let_case tm1 t1 v1 (fst y) (snd y) v2)
+  | Tapp l ts => fun Hsz =>
+    (*Need dependent map for termination proof*)
+    recs <- errst_list (map tm_traverse ts) ;;
+    (app_case tm1 l ts recs)
+  (*Case is the trickiest: we need both a dependent map and a dependent bind*)
+  | Tcase t1 tbs => fun Hsz =>
+    r1 <- tm_traverse t1 ;;
+    tbs2 <- errst_list (map (fun b =>
+      (*Idea: For each element in list, use dependent bind and recursively traverse*)
+        errst_bind_dep (errst_tup1 (errst_lift1 (t_open_branch b)))
+          (fun y s Heq =>
+            t2 <- tm_traverse (snd y) ;;
+            errst_ret (y, t2))
+        ) tbs) ;;
+    match_case tm1 t1 r1 tbs2
+  | Teps b => fun Hsz =>
+    errst_bind_dep (errst_tup1 (errst_lift1 (t_open_bound b)))
+      (fun y s Heq => 
+        v <- (tm_traverse (snd y)) ;;
+        eps_case tm1 (fst y) (snd y) v)
+  (*A slight complication from the triggers - need nested dependent match*)
+  | Tquant q tq => fun Hsz =>
+    (*NOTE: doing bind ... ret, need for proofs even though superflous*)
+    errst_bind_dep (errst_tup1 (errst_lift1 (t_open_quant1 tq)))
+      (fun (y : list vsymbol * trigger * term_c) s Heq => 
+        v <- (tm_traverse (snd y)) ;;
+        let vs := fst (fst y) in
+        let tr := snd (fst y) in
+        let t := snd y in
+        (*Then traverse over triggers*)
+        v2 <- errst_list (map (fun l1 =>
+          errst_list (map tm_traverse l1)) tr) ;;
+        quant_case tm1 q vs tr v2 t v)
+  | Tbinop b t1 t2 => fun Hsz =>
+    r1 <- tm_traverse t1 ;;
+    r2 <- tm_traverse t2 ;;
+    binop_case tm1 b t1 t1 r1 r2
+  | Tnot t1 => fun Hsz =>
+    r1 <- tm_traverse t1 ;;
     not_case tm1 t1 r1
   | Ttrue => fun _ => true_case tm1
   | Tfalse => fun _ => false_case tm1
   end (eq_sym (term_size_eq tm1)).
+Proof.
+  (*Basically, use some sort of proof irrelevance*)
+  unfold tm_traverse at 1.
+  generalize dependent (lt_wf (term_size tm1)).
+  destruct tm1. destruct t; intros ACC; destruct ACC; auto.
+  - (*app*) simpl.
+    f_equal. f_equal.
+    match goal with |- context [dep_map ?f ?l ?H] => generalize dependent H end.
+    simpl in *. generalize dependent (S (sum (map term_size l0))).
+    induction l0; simpl in *; auto. intros n ACC Hall.
+    inversion Hall; subst. f_equal; auto.
+    (*Now use irrelevance*) apply term_traverse_irrel.
+  - (*if*) simpl. unfold tm_traverse.
+    erewrite (term_traverse_irrel t).
+    erewrite (term_traverse_irrel t1).
+    erewrite (term_traverse_irrel t2).
+    reflexivity.
+  - (*let*) simpl.
+    unfold tm_traverse. f_equal.
+    2: { apply term_traverse_irrel. }
+    funext. intros x. f_equal. funext. intros tb.
+    funext. intros s. funext. intros Htb.
+    f_equal. apply term_traverse_irrel.
+  - (*case*) simpl.
+    unfold tm_traverse.
+    f_equal. 2: apply term_traverse_irrel.
+    funext. intros x. f_equal. f_equal.
+    (*inner induction*) gen_dep_map. (*TEMP; bad *) 
+    generalize dependent (@tmatch_size2 St (mk_term_c (Tcase t l) o t0 o0)).
+    Opaque term_traverse. simpl in *. Transparent term_traverse.
+    generalize dependent (S (term_size t + sum (map (fun x1 : pattern_c * bind_info * term_c => term_size (snd x1)) l))).
+    induction l as [|[[p1 b1] t1] ps IH]; auto;
+    intros n a size_bound Hall; auto. inversion Hall; subst.
+    Opaque term_traverse. simpl. Transparent term_traverse. f_equal; auto.
+    f_equal. funext. intros x1. funext. intros s. funext. intros Heq.
+    f_equal. apply term_traverse_irrel.
+  - (*eps*) simpl. f_equal. funext. intros tb. funext. intros s.
+    funext. intros Heq. f_equal. apply term_traverse_irrel.
+  - (*quant*) simpl. destruct p as [[[vs1 b1] tr1] t1]. simpl. f_equal. funext. intros tq.
+    funext. intros s. funext. intros Heq. f_equal. 2: apply term_traverse_irrel.
+    funext. intros x. f_equal. f_equal.
+    (*nested ind*) simpl in *.
+    gen_dep_map. simpl. generalize dependent (S (term_size t1 + Datatypes.length tr1 +
+      sum (map (fun l : list term_c => sum (map term_size l)) tr1))).
+    clear. induction (snd (fst tq)) as [| l1 trs IH]; auto; intros n a Hall; inversion Hall; subst;
+    simpl; f_equal; auto.
+    f_equal. gen_dep_map. clear. induction l1 as [| x1 l1 IH]; auto; simpl; intros Hall; inversion Hall; 
+    subst; f_equal; auto. apply term_traverse_irrel.
+  - (*binop*) simpl. erewrite (term_traverse_irrel t). erewrite (term_traverse_irrel t1); reflexivity.
+  - (*not*) simpl. erewrite (term_traverse_irrel t). reflexivity.
+Qed.
 
-Definition tm_traverse (tm1: term_c) : T :=
-  term_traverse tm1 (Wf_nat.lt_wf _).
+(*With this, we can prove an induction principle*)
 
-
-(*Need an induction principle*)
+(*Have to prove by hand because Equations has bug with monadic binders + well-founded rec*)
 
 Section Induction.
 
-Check tm_traverse.
-Print T.
-Print R.
 Variable (P: term_c -> T -> Prop).
-Check const_case.
+
 Variable (Pconst: forall t c, t_node_of t = Tconst c -> P t (const_case t c)).
 Variable (Pvar: forall t x, t_node_of t = Tvar x -> P t (var_case t x)).
 Variable (Pif: forall t t1 t2 t3, t_node_of t = Tif t1 t2 t3 ->
@@ -186,11 +465,11 @@ Variable (Pquant: forall t q tq, t_node_of t = Tquant q tq ->
         v <- (tm_traverse (snd y)) ;;
         let vs := fst (fst y) in
         let tr := snd (fst y) in
-        let t := snd y in
+        let t' := snd y in
         (*Then traverse over triggers*)
         v2 <- errst_list (map (fun l1 =>
           errst_list (map tm_traverse l1)) tr) ;;
-        quant_case t q vs tr v2 t v))).
+        quant_case t q vs tr v2 t' v))).
 (*Easier*)
 Variable (Pbinop: forall t b t1 t2, t_node_of t = Tbinop b t1 t2 ->
   P t1 (tm_traverse t1) -> P t2 (tm_traverse t2) ->
@@ -202,100 +481,65 @@ Variable (Pnot: forall t t1, t_node_of t = Tnot t1 ->
 Variable (Ptrue: forall t, t_node_of t = Ttrue -> P t (true_case t)).
 Variable (Pfalse: forall t, t_node_of t = Tfalse -> P t (false_case t)).
 
-Lemma tm_size_wf: well_founded (fun t1 t2 => term_size t1 < term_size t2).
-Proof.
-  eapply well_founded_lt_compat with (f:=term_size). auto.
-Defined.
-Set Bullet Behavior "Strict Subproofs".
+(*Prove by well-founded induction on the size of t, use rewrite lemma
+  to avoid dealing with accessibility proofs. Most cases are quite straightforward;
+  relies on the size theorems in TermTraverseAux.v.
+  The quant case is a bit annoying because we need double nested induction *)
 Theorem tm_traverse_ind (t: term_c) : P t (tm_traverse t).
 Proof.
-  (*Idea: do strong induction on size*) (*TODO: proof irrelevance will be terrible, right?*)
-  (*Do we need to unfold definition - assume proof irrelevance if needed*)
   induction t using (well_founded_induction tm_size_wf). rename H into IH.
-  unfold tm_traverse.
+  (*Now use rewrite lemma so we don't need to worry about ACC proofs*)
+  rewrite tm_traverse_rewrite.
+  generalize dependent (eq_sym (term_size_eq t)).
   destruct t as [n tyo a loc].
-  destruct n.
-  - simpl. apply Pvar. reflexivity. 
-  - simpl. apply Pconst. reflexivity.
-  - (*app*)
-    simpl.
+  destruct n; auto.
+  - (*var*) simpl. intros _. apply Pvar. reflexivity.
+  - (*const*) simpl. intros _. apply Pconst. reflexivity.
+  - (*app*) simpl. intros _. apply Papp; auto.
+    (*Use IH to prove the Forall*)
+    simpl in IH. clear -IH. rewrite Forall_forall.
+    intros x Hinx. apply IH. 
+    pose proof (sum_in_lt (map term_size l0) (term_size x)) as Hle.
+    forward Hle. { rewrite in_map_iff. exists x; auto. }
+    lia.
+  - (*if*) simpl. intros _; apply Pif; auto; apply IH; simpl; lia.
+  - (*let*) simpl. destruct p as [[v b] t1]. intros _. apply Plet; auto.
+    + apply IH; simpl; lia.
+    + intros y s Hrun. apply dep_bnd_size_bound' in Hrun.
+      simpl in Hrun. apply IH. simpl. lia.
+  - (*case*) simpl. intros _. apply Pcase; auto.
+    + apply IH; simpl; lia.
+    + rewrite Forall_forall. intros x Hinx y s Hy. apply IH.
+      simpl. apply dep_bnd_size_branch' in Hy. 
+      pose proof (sum_in_lt (map (fun x0 : pattern_c * bind_info * term_c => term_size (snd x0)) l) (term_size (snd x))) as Hle.
+      forward Hle. { rewrite in_map_iff; exists x; auto. } lia.
+  - (*eps*)  destruct p as [[v b] t1].  simpl. intros _; apply Peps; auto.
+    intros y s Hy. apply dep_bnd_size_bound' in Hy. simpl in Hy. apply IH; simpl; lia.
+  - (*quant*) simpl. intros _. apply Pquant; auto.
+    intros y s Hy.
+    apply dep_bnd_size_quant' in Hy.
+    destruct Hy as [Hz1 Hsz2]. destruct p as [[[vs1 b1] tr1] t1].
+    split.
+    + apply IH; simpl in *; lia.
+    + simpl in Hsz2. 
+      (*Forall2 means we need nested induction*)
+      rewrite Forall_forall. intros ts Hints. rewrite Forall_forall.
+      intros x Hinx. apply IH. simpl.
+      assert (Hsz: term_size x <=  sum (map (fun l : list term_c => sum (map term_size l)) tr1)); [|lia].
+      clear -Hsz2 Hints Hinx. generalize dependent tr1. induction (snd (fst y)) as [|l1 tl1 IHl1]; intros [| l2 tl2];
+      simpl; auto; try contradiction; intros Hall; inversion Hall as [| ? ? ? ? IH1 IH2]; subst; clear Hall.
+      simpl in Hints. destruct Hints as [Hts | Hts]; subst; auto.
+      2: { apply IHl1 in IH2; auto. lia. }
+      assert (Hsz: term_size x <= sum (map term_size l2)); [|lia].
+      clear -Hinx IH1. generalize dependent l2. induction ts as [| x1 tl1 IH]; intros [| y2 tl2]; auto; 
+      try contradiction; intros Hall; inversion Hall as [| ? ? ? ? IH1 IH2]; subst. simpl.
+      simpl in Hinx. destruct Hinx; subst; auto; try lia. apply IH in IH2; auto; lia.
+  - (*binop*) simpl. intros _. apply Pbinop; auto; apply IH; simpl; lia.
+  - (*not*) simpl. intros _. apply Pnot; auto; apply IH; simpl; lia.
+Qed.
 
-(*TODO: maybe try equations, might be simpler - just need to do nested induction properly
-  But then we get induction for free*)
+End Induction.
 
-
-  unfold tm_traverse.
-  generalize dependent (lt_wf (term_size t)).
-  
-
-(*As above: new variable, new term, new result*)
-
-Variable (binop_case: forall (tm: term_c) (b: binop) (t1 t2: term_c) (r1 r2: R), T).
-Variable (not_case: forall (tm: term_c) (t: term_c) (r: R), T).
-Variable (true_case: term_c ->T).
-Variable (false_case : term_c ->T).
-
-  | Tbinop b t1 t2 => fun Hsz =>
-    r1 <- term_traverse t1 (Acc_inv ACC (tbinop_size1 Hsz)) ;;
-    r2 <- term_traverse t2 (Acc_inv ACC (tbinop_size2 Hsz)) ;;
-    binop_case tm1 b t1 t1 r1 r2
-  | Tnot t1 => fun Hsz =>
-    r1 <- term_traverse t1 (Acc_inv ACC (tnot_size1 Hsz)) ;;
-    not_case tm1 t1 r1
-  | Ttrue => fun _ => true_case tm1
-  | Tfalse => fun _ => false_case tm1
-
-
-
-
-| Tcase t1 tbs => fun Hsz =>
-    r1 <- term_traverse t1 (Acc_inv ACC (tmatch_size1 Hsz)) ;;
-    tbs2 <- errst_list (@dep_map _ _ (fun x => term_size (snd x) < term_size tm1)
-      (*Idea: For each element in list, use dependent bind and recursively traverse*)
-      (fun b (Hx: term_size (snd b) < term_size tm1) =>
-        errst_bind_dep (errst_tup1 (errst_lift1 (t_open_branch b)))
-          (fun y s Heq =>
-            t2 <- term_traverse (snd y) (Acc_inv ACC (tmatch_size2 Hx Heq)) ;;
-            errst_ret (y, t2))
-        ) tbs (tmatch_size3 Hsz)) ;;
-    match_case tm1 t1 r1 tbs2
-
-
-(*Again, tbs is a list of (new pattern, new term, recursive call)*)
-Variable (match_case: forall (tm: term_c) (t1: term_c) (r1: R) (tb: list (pattern_c * term_c * R)), T).
-
-
-
-Variable (app_case: forall (tm: term_c) (l: lsymbol) (tms: list term_c) (rs: list R), T).
-
-(*TODO: continue*)
-
-
-| Tapp l ts => fun Hsz =>
-    (*Need dependent map for termination proof*)
-    recs <- errst_list (@dep_map _ _ (fun t => term_size t < term_size tm1) 
-      (fun t1 (Ht1: term_size t1 < term_size tm1) => 
-        term_traverse t1 (Acc_inv ACC Ht1)) ts (tapp_size Hsz)) ;;
-    (app_case tm1 l ts recs)
-
-(*tm_traverse_elim
-     : forall P : tm -> ctr T -> Type,
-       (forall c : CoqBigInt.t, P (Tconst c) (const_case c)) ->
-       (forall x : var, P (Tvar x) (var_case x)) ->
-       (forall (o : intop) (t1 t2 : tm),
-        (T -> P t2 (tm_traverse t2)) ->
-        P t1 (tm_traverse t1) ->
-        P (Top o t1 t2) (v1 <- tm_traverse t1;; v2 <- tm_traverse t2;; op_case o t1 t2 v1 v2)) ->
-       (forall (t1 : tm) (b : var * tm),
-        (T ->
-         forall (y : var * tm) (s : CoqBigInt.t),
-         y = fst (runState (t_open_bound b) s) -> P (snd y) (tm_traverse (snd y))) ->
-        P t1 (tm_traverse t1) ->
-        P (Tlet t1 b)
-          (v1 <- tm_traverse t1;;
-           y <-- s <-- _ <-- t_open_bound b;;
-           v2 <- tm_traverse (snd y);; let_case t1 (fst y, snd b) v1 v2)) ->
-       forall tm1 : tm, P tm1 (tm_traverse tm1)*)
 
 End Traverse.
 
